Fix some broken files -- now compiles without StaticMutrecAproof

bound/LinkingC2.v
@@ -1,4 +1,4 @@
-Require Import Coqlib Maps Errors AST Linking LinkingC sflib.
+Require Import CoqlibC Maps Errors AST Linking LinkingC sflib.
 
 Remark link_transf_partial_fundef_rev:
   forall (A B: Type) (tr1 tr2: A -> res B) (f1 f2: fundef A) (tf1 tf2: fundef B) (tf: fundef B),
@@ -137,3 +137,98 @@ Section LINK_LIST_MATCH.
   Qed.
 
 End LINK_LIST_MATCH.
+
+Require Import CtypesC CsemC.
+
+(* Copied from CtypesC. The only difference is it checks type on external-internal function linking *)
+
+Definition link_fundef (fd1 fd2: fundef) :=
+  match fd1, fd2 with
+  | Internal _, Internal _ => None
+  | External ef1 targs1 tres1 cc1, External ef2 targs2 tres2 cc2 =>
+      if external_function_eq ef1 ef2
+      && typelist_eq targs1 targs2
+      && type_eq tres1 tres2
+      && calling_convention_eq cc1 cc2
+      then Some (External ef1 targs1 tres1 cc1)
+      else None
+  | Internal f, External ef targs tres cc =>
+    if (list_eq_dec type_eq f.(fn_params).(map snd) targs.(typelist_to_listtype))
+         && (type_eq f.(fn_return) tres)
+         && (calling_convention_eq f.(fn_callconv) cc)
+    then
+      match ef with EF_external id sg => if signature_eq (signature_of_type targs tres cc) sg then Some (Internal f) else None | _ => None end
+    else None
+  | External ef targs tres cc, Internal f =>
+    if (list_eq_dec type_eq f.(fn_params).(map snd) targs.(typelist_to_listtype))
+         && (type_eq f.(fn_return) tres)
+         && (calling_convention_eq f.(fn_callconv) cc)
+    then
+      match ef with EF_external id sg => if signature_eq (signature_of_type targs tres cc) sg then Some (Internal f) else None | _ => None end
+    else None
+  end.
+
+Inductive linkorder_fundef: fundef -> fundef -> Prop :=
+  | linkorder_fundef_refl: forall fd,
+      linkorder_fundef fd fd
+  | linkorder_fundef_ext_int: forall f id sg targs tres cc,
+      linkorder_fundef (External (EF_external id sg) targs tres cc) (Internal f).
+
+Instance Linker_fundef: Linker (fundef) := {
+  link := link_fundef;
+  linkorder := linkorder_fundef
+}.
+Proof.
+- intros; constructor.
+- intros. inv H; inv H0; constructor.
+- intros x y z EQ. destruct x, y; simpl in EQ.
++ discriminate.
++ des_ifs. split; constructor.
++ des_ifs. split; constructor.
++ des_ifs. bsimpl. des. des_sumbool. clarify. split; constructor.
+Defined.
+
+Definition link_program (p1 p2: program): option (program) :=
+  match link (program_of_program p1) (program_of_program p2) with
+  | None => None
+  | Some p =>
+      match lift_option (link p1.(prog_types) p2.(prog_types)) with
+      | inright _ => None
+      | inleft (exist typs EQ) =>
+          match link_build_composite_env
+                   p1.(prog_types) p2.(prog_types) typs
+                   p1.(prog_comp_env) p2.(prog_comp_env)
+                   p1.(prog_comp_env_eq) p2.(prog_comp_env_eq) EQ with
+          | exist env (conj P Q) =>
+              Some {| prog_defs := p.(AST.prog_defs);
+                      prog_public := p.(AST.prog_public);
+                      prog_main := p.(AST.prog_main);
+                      prog_types := typs;
+                      prog_comp_env := env;
+                      prog_comp_env_eq := P |}
+          end
+      end
+  end.
+
+Definition linkorder_program (p1 p2: program) : Prop :=
+     linkorder (program_of_program p1) (program_of_program p2)
+  /\ (forall id co, p1.(prog_comp_env)!id = Some co -> p2.(prog_comp_env)!id = Some co).
+
+Instance Linker_program: Linker (program) := {
+  link := link_program;
+  linkorder := linkorder_program
+}.
+Proof.
+- intros; split. apply linkorder_refl. auto. 
+- intros. destruct H, H0. split. eapply linkorder_trans; eauto.
+  intros; auto.
+- intros until z. unfold link_program. 
+  destruct (link (program_of_program x) (program_of_program y)) as [p|] eqn:LP; try discriminate.
+  destruct (lift_option (link (prog_types x) (prog_types y))) as [[typs EQ]|EQ]; try discriminate.
+  destruct (link_build_composite_env (prog_types x) (prog_types y) typs
+       (prog_comp_env x) (prog_comp_env y) (prog_comp_env_eq x)
+       (prog_comp_env_eq y) EQ) as (env & P & Q & R).
+  destruct (link_linkorder _ _ _ LP). 
+  intros X; inv X.
+  split; split; auto.
+Defined.
